Fix a proof in Spec.SHA2.Lemmas

specs/lemmas/Spec.SHA2.Lemmas.fst
@@ -6,9 +6,12 @@ module S = FStar.Seq
 
 open Spec.Hash.Definitions
 open Spec.SHA2
+open Spec.Hash.Lemmas
 
 friend Spec.SHA2
 friend Spec.Agile.Hash
+
+#set-options "--z3rlimit 25 --fuel 0 --ifuel 0"
 
 (* Scheduling function *)
 
@@ -215,12 +218,30 @@ let update_224_256 hash block =
 
 #pop-options
 
-
 let rec update_multi_224_256 hash blocks =
-  assert_norm (words_state SHA2_224 == words_state SHA2_256);
+  let a = SHA2_256 in
+  let a' = SHA2_224 in
+  assert_norm (words_state a == words_state a');
   if S.length blocks = 0 then
-    ()
+    begin
+    assert(blocks `S.equal` S.empty);
+    Spec.Hash.Lemmas.update_multi_zero a hash;
+    Spec.Hash.Lemmas.update_multi_zero a' hash
+    end
   else
-    let block, rem = Lib.UpdateMulti.split_block (block_length SHA2_256) blocks 1 in
-    update_224_256 hash block;
-    update_multi_224_256 (update SHA2_224 hash block) rem
+    begin
+    assert(block_length a = block_length a');
+    let block1, blocks_end = S.split blocks (block_length a) in
+    assert(S.length block1 = block_length a);
+    assert(S.length blocks_end % block_length a = 0);
+    assert(S.append block1 blocks_end `S.equal` blocks);
+    update_multi_associative a hash block1 blocks_end;
+    update_multi_associative a' hash block1 blocks_end;
+    update_multi_update a hash block1;
+    update_multi_update a' hash block1;
+    let hash1 = Spec.Agile.Hash.update a hash block1 in
+    let hash2 = Spec.Agile.Hash.update a' hash block1 in
+    update_224_256 hash block1;
+    assert(hash1 == hash2);
+    update_multi_224_256 hash1 blocks_end
+    end
